We are interested in integral
$$I = \int_{-\infty}^{\infty} \dd{\epsilon} H(\epsilon) n_F(\epsilon) $$

Define
$$K(\epsilon) = \int_{-\infty}^{\epsilon} \dd{\epsilon'} H(\epsilon') $$

Integrating by parts:
$$I = \underbrace{\eval{K(\epsilon ) n_F(\epsilon)}_{-\infty}^{\infty}}_{0} +\int_{-\infty}^\infty K(\epsilon) \qty(-\pdv{n_F}{\epsilon}) $$

Now
$$-\pdv{n_F}{\epsilon} = \frac{\beta e^{\beta\qty(\epsilon-\mu)}}{\qty( e^{\beta\qty(\epsilon-\mu)}+1)^2} = \frac{\beta}{4\cosh(\frac{\beta(\epsilon-\mu)}{2})}$$
Note that
$$\int_{-\infty}^\infty \dd{\epsilon} \qty(-\pdv{n_F}{\epsilon}) =1$$

Now we want to take Taylor series of $K$:

$$K(\epsilon) = K(\mu) + \sum_n \frac{(\epsilon-\mu)^n}{n!} \dv[n]{k}{\epsilon} \qty(\mu)$$

i.e.,
$$I = K(\mu)\int_{-\infty}^\infty \dd{\epsilon} \qty(\pdv{n_F}{\epsilon}) + \sum_n \int_{-\infty}^\infty \dd{\epsilon}  \frac{(\epsilon-\mu)^{2n}}{(2n)!} \qty[-\pdv{n_F}{\epsilon}] \dv[2n]{K}{\epsilon} \qty(\mu)$$

Define $x=\beta(\epsilon-\mu)$:
$$\int_{-\infty}^\infty \dd{\epsilon}  \frac{(\epsilon-\mu)^{2n}}{(2n)!} \qty[-\pdv{n_F}{\epsilon}] \dv[2n]{K}{\epsilon} \qty(\mu) = (k_BT)^{2n}\int_{-\infty}^\infty \dd{x} r_n(x) \dv[2n]{K}{\epsilon} \qty(\mu)$$

Define
$$a_n = \int_{-\infty}^\infty \dd{x} r_n(x) = \int_{-\infty}^\infty \dd{x} \frac{x^{2n}}{(2n)!} \qty(-\dv{x} \frac{1}{e^x+1})$$
We can get
$$a_n = \qty(2-\frac{1}{2^{2(n+1)}}) \zeta(2n)$$


Thus
$$I = \int_{-\infty}^\mu H(\epsilon) \dd{\epsilon} + \frac{\pi^2}{6} (kT)^2 H'(\mu) + \frac{7\pi^4}{360} (k_BT)^4 H^{(3)} (\mu) + \order{(k_BT)^6} $$

\paragraph{Chemical potential in low temperatures}
$$n = \int_{-\infty}^\infty g(\epsilon) n_F(\beta(\epsilon-\mu))$$
$$n = \underbrace{\int_{-\infty}^\mu g(\epsilon) \dd{\epsilon}}_{n} + \frac{\pi^2}{6} (kT)^2 g'(\mu)$$
Doing Taylors again:
$$\int_{-\infty}^\mu g(\epsilon) \dd{\epsilon} = \int_{-\infty}^{\epsilon_F} g(\epsilon) \dd{\epsilon} + (\mu-\epsilon_F) g(\epsilon_F)$$
$$g'(\mu) = g'(\epsilon_F) + (\mu-\epsilon_F) g''(\epsilon_F)$$

Thus
$$n = n + (\mu-\epsilon_F) g(\epsilon_F) + \frac{\pi^2}{6} (kT)^2 g'(\epsilon_F)$$
and
$$\mu = \epsilon_F - \frac{\pi^2}{6} (kT)^2 \frac{g'(\epsilon_F)}{g(\epsilon_F)} $$

\paragraph{Energy}
\begin{align*}
\expval{E} = \int_{-\infty}^\mu \dd{\epsilon} g(\epsilon) \epsilon + \frac{\pi^2}{6} (k_BT)^2 \qty(g(\mu) + g'(\mu) \mu ) =\\= \int_{-\infty}^{\epsilon_F} \dd{\epsilon} g(\epsilon) \epsilon + (\mu-\epsilon_F) g(\epsilon_F) \epsilon_F + \frac{\pi^2}{6} (k_BT)^2 \frac{g'(\epsilon_F)}{g(\epsilon_F)} g(\epsilon_F)\epsilon_F + \frac{\pi^2}{6} (k_BT)^2 \qty(g(\epsilon_F) + g'(\epsilon_F)\epsilon_F)
\end{align*}
$$ \expval{E} = \expval{E}(T=0) + \frac{\pi^2}{6} (k_BT)^2 g(\epsilon_F)  $$